experiment: use plaisted-greenbaum encoding to CNF

src/Std/Sat/AIG/CNF.lean
@@ -33,35 +33,29 @@ def falseToCNF (output : α) : CNF α :=
 /--
 Produce a Tseitin style CNF for a `Decl.atom`, using `output` as the tree node variable.
 -/
-def atomToCNF (output : α) (atom : α) : CNF α :=
+def atomToCNF (output : Nat) (atom : Nat) : CNF Nat :=
   CNF.empty
     |>.add (CNF.Clause.empty |>.add output .true |>.add atom .false)
     |>.add (CNF.Clause.empty |>.add output .false |>.add atom .true)
 
-/--
-Produce a Tseitin style CNF for a `Decl.gate`, using `output` as the tree node variable.
--/
-def gateToCNF (output : α) (lhs rhs : α) (linv rinv : Bool) : CNF α :=
-  -- a ↔ (b and c) as CNF: (¬a ∨ b) ∧ (¬a ∨ c) ∧ (a ∨ ¬b ∨ ¬c)
-  -- a ↔ (b and ¬c) as CNF: (¬a ∨ b) ∧ (¬a ∨ ¬c) ∧ (a ∨ ¬b ∨ c)
-  -- a ↔ (¬b and c) as CNF: (¬a ∨ ¬b) ∧ (¬a ∨ c) ∧ (a ∨ b ∨ ¬c)
-  -- a ↔ (¬b and ¬c) as CNF: (¬a ∨ ¬b) ∧ (¬a ∨ ¬c) ∧ (a ∨ b ∨ c)
+def gatePosToCNF (output : Nat) (lhs rhs : Nat) (linv rinv : Bool) : CNF Nat :=
   CNF.empty
     |>.add (CNF.Clause.empty |>.add output .false |>.add lhs !linv)
     |>.add (CNF.Clause.empty |>.add output .false |>.add rhs !rinv)
+
+def gateNegToCNF (output : Nat) (lhs rhs : Nat) (linv rinv : Bool) : CNF Nat :=
+  CNF.empty
     |>.add (CNF.Clause.empty |>.add output .true |>.add lhs linv |>.add rhs rinv)
 
-/--
-Produce a Tseitin style CNF for an if-then-else gate, using `output` as the tree node variable.
--/
-def iteToCNF (output : α) (cond ifTrue ifFalse : α) (cinv tinv finv : Bool) : CNF α :=
-  -- o ↔ (c ? t : f) as implications: (c ∧ t → o) ∧ (c ∧ ¬t → ¬o) ∧ (¬c ∧ f → o) ∧ (¬c ∧ ¬f → ¬o)
-  -- o ↔ (c ? t : f) as CNF: (¬c ∨ ¬t ∨ o) ∧ (¬c ∨ t ∨ ¬o) ∧ (c ∨ ¬f ∨ o) ∧ (c ∨ f ∨ ¬o)
+def itePosToCNF (output : Nat) (cond ifTrue ifFalse : Nat) (cinv tinv finv : Bool) : CNF Nat :=
+  CNF.empty
+    |>.add (CNF.Clause.empty |>.add cond cinv |>.add ifTrue !tinv |>.add output .false)
+    |>.add (CNF.Clause.empty |>.add cond !cinv |>.add ifFalse !finv |>.add output .false)
+
+def iteNegToCNF (output : Nat) (cond ifTrue ifFalse : Nat) (cinv tinv finv : Bool) : CNF Nat :=
   CNF.empty
     |>.add (CNF.Clause.empty |>.add cond cinv |>.add ifTrue tinv |>.add output .true)
-    |>.add (CNF.Clause.empty |>.add cond cinv |>.add ifTrue !tinv |>.add output .false)
     |>.add (CNF.Clause.empty |>.add cond !cinv |>.add ifFalse finv |>.add output .true)
-    |>.add (CNF.Clause.empty |>.add cond !cinv |>.add ifFalse !finv |>.add output .false)
 
 @[simp]
 theorem falseToCNF_eval :
@@ -79,27 +73,74 @@ theorem atomToCNF_eval :
     CNF.Clause.eval_empty, Bool.or_false, CNF.eval_empty, Bool.and_true]
   cases assign output <;> cases assign a <;> decide
 
+-- This ensures output is still false when it should be
 @[simp]
+theorem gatePosToCNF_eval :
+    (gatePosToCNF output lhs rhs linv rinv).eval assign
+      =
+    decide ((((assign lhs) ^^ linv) && ((assign rhs) ^^ rinv)) ≥ assign output) := by
+  simp [gatePosToCNF]
+  generalize assign lhs = l
+  generalize assign rhs = r
+  generalize assign output = o
+  decide +revert
+
+-- This ensures output is still true when it should be
+@[simp]
+theorem gateNegToCNF_eval :
+    (gateNegToCNF output lhs rhs linv rinv).eval assign
+      =
+    decide ((((assign lhs) ^^ linv) && ((assign rhs) ^^ rinv)) ≤ assign output) := by
+  simp [gateNegToCNF]
+  generalize assign lhs = l
+  generalize assign rhs = r
+  generalize assign output = o
+  decide +revert
+
 theorem gateToCNF_eval :
-    (gateToCNF output lhs rhs linv rinv).eval assign
+    ((gatePosToCNF output lhs rhs linv rinv) ++ (gateNegToCNF output lhs rhs linv rinv)).eval assign
       =
     (assign output == (((assign lhs) ^^ linv) && ((assign rhs) ^^ rinv))) := by
-  simp only [gateToCNF, CNF.eval_add, CNF.Clause.eval_add, beq_true, CNF.Clause.eval_empty,
-    Bool.or_false, beq_false, CNF.eval_empty, Bool.and_true]
-  cases assign output
-    <;> cases assign lhs
-      <;> cases assign rhs
-        <;> cases linv
-          <;> cases rinv
-            <;> decide
+  simp [gatePosToCNF_eval, gateNegToCNF_eval]
+  generalize assign lhs = l
+  generalize assign rhs = r
+  generalize assign output = o
+  decide +revert
 
 @[simp]
+theorem itePosToCNF_eval {cond ifTrue ifFalse cinv tinv finv assign} :
+    (itePosToCNF output cond ifTrue ifFalse cinv tinv finv).eval assign
+      =
+    decide
+      ((ite ((assign cond) ^^ cinv) ((assign ifTrue) ^^ tinv) ((assign ifFalse) ^^ finv)) ≥
+        assign output) := by
+  simp [itePosToCNF]
+  generalize assign output = o
+  generalize assign cond = c
+  generalize assign ifTrue = t
+  generalize assign ifFalse = f
+  decide +revert
+
+@[simp]
+theorem iteNegToCNF_eval {cond ifTrue ifFalse cinv tinv finv assign} :
+    (iteNegToCNF output cond ifTrue ifFalse cinv tinv finv).eval assign
+      =
+    decide
+      ((ite ((assign cond) ^^ cinv) ((assign ifTrue) ^^ tinv) ((assign ifFalse) ^^ finv)) ≤
+        assign output) := by
+  simp [iteNegToCNF]
+  generalize assign output = o
+  generalize assign cond = c
+  generalize assign ifTrue = t
+  generalize assign ifFalse = f
+  decide +revert
+
 theorem iteToCNF_eval {cond ifTrue ifFalse cinv tinv finv assign} :
-    (iteToCNF output cond ifTrue ifFalse cinv tinv finv).eval assign
+    ((itePosToCNF output cond ifTrue ifFalse cinv tinv finv) ++
+      (iteNegToCNF output cond ifTrue ifFalse cinv tinv finv)).eval assign
       =
     (assign output == ite ((assign cond) ^^ cinv) ((assign ifTrue) ^^ tinv) ((assign ifFalse) ^^ finv)) := by
-  simp only [iteToCNF, CNF.eval_add, CNF.Clause.eval_add, beq_false, CNF.Clause.eval_empty,
-    Bool.or_false, beq_true, CNF.eval_empty, Bool.and_true, bne_iff_ne, ne_eq, ite_not]
+  simp [itePosToCNF_eval, iteNegToCNF_eval]
   generalize assign output = o
   generalize assign cond = c
   generalize assign ifTrue = t
@@ -165,6 +206,229 @@ theorem satAssignment_inr (h : x < aig.decls.size) :
     (cnfSatAssignment aig assign1) x = ⟦aig, ⟨x, false, h⟩, assign1⟧ := by
   simp [cnfSatAssignment, mixAssigns, h]
 
+inductive BiMark where
+| bottom
+| uninverted
+| inverted
+| top
+
+namespace BiMark
+
+@[inline]
+def has (inversion : Bool) : BiMark → Bool
+| bottom => false
+| uninverted => !inversion
+| inverted => inversion
+| top => true
+
+@[simp]
+theorem has_bottom :
+    has inversion bottom = false := by
+  simp [has]
+
+@[simp]
+theorem has_uninverted :
+    has inversion uninverted = !inversion := by
+  simp [has]
+
+@[simp]
+theorem has_inverted :
+    has inversion inverted = inversion := by
+  simp [has]
+
+@[simp]
+theorem has_top :
+    has inversion top = true := by
+  simp [has]
+
+theorem ext_iff {a b : BiMark} :
+    a = b ↔ (a.has false = b.has false) ∧ (a.has true = b.has true) := by
+  cases a <;> cases b <;> simp
+
+instance instLE : LE BiMark where
+  le a b := (a.has false ≤ b.has false) ∧ (a.has true ≤ b.has true)
+
+theorem le_iff {a b : BiMark} :
+    a ≤ b ↔ (a.has false ≤ b.has false) ∧ (a.has true ≤ b.has true) := by
+  rfl
+
+@[inline]
+instance : DecidableLE BiMark := by
+  simp +instances only [instLE, DecidableLE]
+  infer_instance
+
+@[simp]
+theorem le_rfl {a : BiMark} :
+    a ≤ a := by
+  simp +instances only [instLE]
+  simp [has]
+
+theorem le_trans {a b c : BiMark} :
+    a ≤ b → b ≤ c → a ≤ c := by
+  simp +instances only [instLE, has]
+  cases a <;> cases b <;> cases c
+  <;> simp
+
+@[simp]
+theorem le_top :
+    a ≤ top := by
+  simp [le_iff]
+
+@[simp]
+theorem top_le :
+    top ≤ a ↔ a = top := by
+  constructor
+  · simp +instances only [instLE, has]
+    cases a <;> simp [show ¬(true ≤ false) by decide] <;> trivial
+  · intro h
+    simp [h]
+
+@[simp]
+theorem bottom_le :
+    bottom ≤ a := by
+  simp [le_iff]
+
+theorem has_of_le {a b : BiMark} {inv : Bool} :
+    a ≤ b → a.has inv → b.has inv := by
+  simp only [le_iff, and_imp]
+  cases inv
+  <;> generalize has false a = hfa
+  <;> generalize has true a = hfa
+  <;> generalize has false b = hfb
+  <;> generalize has true b = htb
+  <;> decide +revert
+
+@[inline]
+def of (invert : Bool) : BiMark :=
+  if invert then .inverted else uninverted
+
+@[simp]
+theorem has_of :
+    has inversion (of invert) = (inversion = invert) := by
+  simp [of]
+  split <;> simp_all
+
+@[inline]
+def join : BiMark → BiMark → BiMark
+| bottom, other
+| other, bottom => other
+| uninverted, uninverted => uninverted
+| inverted, inverted => inverted
+| _, _ => top
+
+@[simp]
+theorem has_join :
+    (join a b).has inversion = (a.has inversion || b.has inversion) := by
+  simp only [has, join]
+  cases a
+  <;> cases b
+  <;> simp
+
+@[simp]
+theorem le_join_left :
+    a ≤ (join a b) := by
+  simp only [le_iff, has_join]
+  cases has false a
+  <;> cases has true a
+  <;> simp
+
+@[simp]
+theorem le_join_right :
+    b ≤ (join a b) := by
+  simp only [le_iff, has_join]
+  cases has false b
+  <;> cases has true b
+  <;> simp
+
+@[simp]
+theorem join_le (ha : a ≤ o) (hb : b ≤ o) :
+    (join a b) ≤ o := by
+  revert ha hb
+  simp only [le_iff, has_join]
+  generalize has false a = hfa
+  generalize has false b = hfb
+  generalize has false o = hfo
+  generalize has true a = hta
+  generalize has true b = htb
+  generalize has true o = hto
+  decide +revert
+
+@[inline]
+def meet : BiMark → BiMark → BiMark
+| top, other
+| other, top => other
+| uninverted, uninverted => uninverted
+| inverted, inverted => inverted
+| _, _ => bottom
+
+@[simp]
+theorem has_meet :
+    (meet a b).has inversion = (a.has inversion && b.has inversion) := by
+  simp only [has, meet]
+  cases a
+  <;> cases b
+  <;> simp
+
+@[simp]
+theorem meet_le_left :
+    (meet a b) ≤ a := by
+  simp only [le_iff, has_meet]
+  cases has false a
+  <;> cases has true a
+  <;> simp
+
+@[simp]
+theorem meet_le_right :
+    (meet a b) ≤ b := by
+  simp only [le_iff, has_meet]
+  cases has false a
+  <;> cases has true a
+  <;> simp
+
+@[inline]
+def invert : BiMark → Bool → BiMark
+| uninverted, true => inverted
+| inverted, true => uninverted
+| a, _ => a
+
+@[simp]
+theorem has_invert :
+    (invert a inv).has inversion = a.has (inversion ^^ inv) := by
+  simp only [has, invert]
+  cases a
+  <;> cases inv
+  <;> simp
+
+@[inline]
+def sub : BiMark → BiMark → BiMark
+| a, bottom => a
+| _, top
+| bottom, _
+| uninverted, uninverted
+| inverted, inverted => bottom
+| _, uninverted => inverted
+| _, inverted => uninverted
+
+@[simp]
+theorem has_sub :
+    (sub a b).has inversion = (a.has inversion && !b.has inversion) := by
+  simp only [has, sub]
+  cases a
+  <;> cases b
+  <;> simp
+
+@[simp]
+theorem join_sub :
+    join (sub a b) b = join a b := by
+  simp [ext_iff]
+  generalize has false a = hfa
+  generalize has false b = hfb
+  generalize has true a = hta
+  generalize has true b = htb
+  decide +revert
+
+end BiMark
+
 /--
 The central invariant for the `Cache`.
 
@@ -175,19 +439,20 @@ This means that if the CNF is satisfiable at some assignment, we can evaluate th
 the atom part of that assignment and will get the value that was assigned to the corresponding
 auxiliary variable as a result.
 -/
-def Cache.Inv (aig : AIG Nat) (cnf : CNF Nat) (marks : Array Bool)
+def Cache.Inv (aig : AIG Nat) (cnf : CNF Nat) (marks : Array BiMark)
     (hmarks : marks.size = aig.decls.size) : Prop :=
-  ∀ (assign : Nat → Bool) (_heval : cnf.eval assign = true) (idx : Nat)
-    (hbound : idx < aig.decls.size) (_hmark : marks[idx]'(by omega) = true),
-      ⟦aig, ⟨idx, false, hbound⟩, projectLeftAssign aig assign⟧ = (projectRightAssign assign) idx
-
+  ∀ (assign : Nat → Bool) (_heval : cnf.eval assign = true) (idx : Nat) (inverted : Bool)
+    (hbound : idx < aig.decls.size) (_hmark : marks[idx]'(by omega) |>.has inverted),
+      (((projectRightAssign assign) idx) ^^ inverted)
+        ≤
+      ⟦aig, ⟨idx, inverted, hbound⟩, projectLeftAssign aig assign⟧
 
 /--
 The `Cache` invariant always holds for an empty CNF when all nodes are unmarked.
 -/
-theorem Cache.Inv_init : Inv aig .empty (.replicate aig.decls.size false)
+theorem Cache.Inv_init : Inv aig .empty (.replicate aig.decls.size .bottom)
     (by simp) := by
-  intro assign _ idx hbound hmark
+  intro assign _ idx inverted hbound hmark
   simp at hmark
 
 /--
@@ -198,7 +463,7 @@ structure Cache (aig : AIG Nat) (cnf : CNF Nat) where
   /--
   Keeps track of AIG nodes that we already turned into CNF.
   -/
-  marks : Array Bool
+  marks : Array BiMark
   /--
   There are always as many marks as AIG nodes.
   -/
@@ -212,69 +477,88 @@ structure Cache (aig : AIG Nat) (cnf : CNF Nat) where
 We say that a cache extends another by an index when it doesn't invalidate any entry and has an
 entry for that index.
 -/
-structure Cache.IsExtensionBy (cache1 : Cache aig cnf1) (cache2 : Cache aig cnf2) (new : Nat)
+structure Cache.IsExtensionBy (cache1 : Cache aig cnf1) (cache2 : Cache aig cnf2) (new : Nat) (mark : BiMark)
     (hnew : new < aig.decls.size) : Prop where
   /--
   No entry is invalidated.
   -/
   extension : ∀ (idx : Nat) (hidx : idx < aig.decls.size),
-                cache1.marks[idx]'(by have := cache1.hmarks; omega) = true
-                  →
-                cache2.marks[idx]'(by have := cache2.hmarks; omega) = true
+                cache1.marks[idx]'(by have := cache1.hmarks; omega) ≤
+                cache2.marks[idx]'(by have := cache2.hmarks; omega)
   /--
   The second cache is true at the new index.
   -/
-  trueAt : cache2.marks[new]'(by have := cache2.hmarks; omega) = true
+  trueAt : mark ≤ cache2.marks[new]'(by have := cache2.hmarks; omega)
 
 theorem Cache.IsExtensionBy_trans_left (cache1 : Cache aig cnf1) (cache2 : Cache aig cnf2)
-    (cache3 : Cache aig cnf3) (h12 : IsExtensionBy cache1 cache2 new1 hnew1)
-    (h23 : IsExtensionBy cache2 cache3 new2 hnew2) : IsExtensionBy cache1 cache3 new1 hnew1 := by
+    (cache3 : Cache aig cnf3) (h12 : IsExtensionBy cache1 cache2 new1 mark1 hnew1)
+    (h23 : IsExtensionBy cache2 cache3 new2 mark2 hnew2) : IsExtensionBy cache1 cache3 new1 mark1 hnew1 := by
   apply IsExtensionBy.mk
-  · intro idx hidx hmarked
-    apply h23.extension
-    · apply h12.extension
-      · exact hmarked
-      · omega
-    · omega
-  · apply h23.extension
-    · exact h12.trueAt
-    · omega
+  · intro idx hidx
+    exact BiMark.le_trans (h12.extension idx hidx) (h23.extension idx hidx)
+  · exact BiMark.le_trans (h12.trueAt) (h23.extension new1 hnew1)
 
 theorem Cache.IsExtensionBy_trans_right (cache1 : Cache aig cnf1) (cache2 : Cache aig cnf2)
-    (cache3 : Cache aig cnf3) (h12 : IsExtensionBy cache1 cache2 new1 hnew1)
-    (h23 : IsExtensionBy cache2 cache3 new2 hnew2) : IsExtensionBy cache1 cache3 new2 hnew2 := by
+    (cache3 : Cache aig cnf3) (h12 : IsExtensionBy cache1 cache2 new1 mark1 hnew1)
+    (h23 : IsExtensionBy cache2 cache3 new2 mark2 hnew2) : IsExtensionBy cache1 cache3 new2 mark2 hnew2 := by
   apply IsExtensionBy.mk
-  · intro idx hidx hmarked
-    apply h23.extension
-    · apply h12.extension
-      · exact hmarked
-      · omega
-    · omega
+  · intro idx hidx
+    exact BiMark.le_trans (h12.extension idx hidx) (h23.extension idx hidx)
   · exact h23.trueAt
 
 /--
 Cache extension is a reflexive relation.
 -/
-theorem Cache.IsExtensionBy_rfl (cache : Cache aig cnf) {h} (hmarked : cache.marks[idx]'h = true) :
-    Cache.IsExtensionBy cache cache idx (have := cache.hmarks; omega) := by
+theorem Cache.IsExtensionBy_rfl (cache : Cache aig cnf) {h}
+    (hmarked : mark ≤ cache.marks[idx]'h) :
+    Cache.IsExtensionBy cache cache idx mark (have := cache.hmarks; omega) := by
   apply IsExtensionBy.mk
-  · intros
-    assumption
+  · simp
   · exact hmarked
 
-theorem Cache.IsExtensionBy_set (cache1 : Cache aig cnf1) (cache2 : Cache aig cnf2) (idx : Nat)
-    (hbound : idx < cache1.marks.size) (h : cache2.marks = cache1.marks.set idx true) :
-    IsExtensionBy cache1 cache2 idx (by have := cache1.hmarks; omega) := by
+theorem Cache.IsExtensionBy_le (cache1 : Cache aig cnf1) (cache2 : Cache aig cnf2) {h}
+    (h12 : Cache.IsExtensionBy cache1 cache2 idx mark1 h) (hle : mark2 ≤ mark1) :
+    Cache.IsExtensionBy cache1 cache2 idx mark2 hnew := by
   apply IsExtensionBy.mk
-  · intro idx hidx hmark
-    simp [Array.getElem_set, hmark, h]
+  · exact h12.extension
+  · exact BiMark.le_trans hle h12.trueAt
+
+theorem Cache.IsExtensionBy_join {cache1 : Cache aig cnf1} {cache2 : Cache aig cnf2} {h}
+    (h1 : Cache.IsExtensionBy cache1 cache2 idx mark1 h)
+    (h2 : Cache.IsExtensionBy cache1 cache2 idx mark2 h)
+    (hjoin : mark3 ≤ mark1.join mark2) :
+    Cache.IsExtensionBy cache1 cache2 idx mark3 hnew := by
+  apply IsExtensionBy.mk
+  · exact h1.extension
+  · apply BiMark.le_trans hjoin
+    exact BiMark.join_le h1.trueAt h2.trueAt
+
+theorem Cache.IsExtensionBy_set (cache1 : Cache aig cnf1) (cache2 : Cache aig cnf2) (idx : Nat)
+    (mark : BiMark) (hbound : idx < cache1.marks.size)
+    (h : cache2.marks = cache1.marks.set idx mark)
+    (hle : cache1.marks[idx]'hbound ≤ mark) :
+    IsExtensionBy cache1 cache2 idx mark (by have := cache1.hmarks; omega) := by
+  apply IsExtensionBy.mk
+  · intro idx hidx
+    simp only [Array.getElem_set, h]
+    split <;> simp_all
   · simp [h]
+
+theorem Cache.IsExtensionBy_modify (cache1 : Cache aig cnf1) (cache2 : Cache aig cnf2) (idx : Nat)
+    (mark : BiMark) (hbound : idx < cache1.marks.size)
+    (h : cache2.marks = cache1.marks.modify idx (·.join mark)) :
+    IsExtensionBy cache1 cache2 idx mark (by have := cache1.hmarks; omega) := by
+  apply IsExtensionBy.mk
+  · intro idx hidx
+    simp only [Array.getElem_modify, h]
+    split <;> simp
+  · simp [h, Array.getElem_modify]
 
 /--
 A cache with no entries is valid for an empty CNF.
 -/
 def Cache.init (aig : AIG Nat) : Cache aig .empty where
-  marks := .replicate aig.decls.size false
+  marks := .replicate aig.decls.size .bottom
   hmarks := by simp
   inv := Inv_init
 
@@ -286,15 +570,15 @@ def Cache.addFalse (cache : Cache aig cnf) (idx : Nat) (h : idx < aig.decls.size
     {
       out : Cache aig (cnf ++ Decl.falseToCNF idx)
         //
-      Cache.IsExtensionBy cache out idx h
+      Cache.IsExtensionBy cache out idx .top h
     } :=
   have hmarkbound : idx < cache.marks.size := by have := cache.hmarks; omega
   let out :=
     { cache with
-      marks := cache.marks.set idx true
+      marks := cache.marks.set idx .top
       hmarks := by simp [cache.hmarks]
       inv := by
-        intro assign heval idx hbound hmarked
+        intro assign heval idx inverted hbound hmarked
         rw [Array.getElem_set] at hmarked
         split at hmarked
         next heq =>
@@ -302,10 +586,10 @@ def Cache.addFalse (cache : Cache aig cnf) (idx : Nat) (h : idx < aig.decls.size
           simp [denote_idx_false htip, heval]
         next heq =>
           simp only [CNF.eval_append, Decl.falseToCNF_eval, Bool.and_eq_true, beq_iff_eq] at heval
-          have := cache.inv assign heval.left idx hbound hmarked
-          rw [this]
+          have := cache.inv assign heval.left idx inverted hbound hmarked
+          apply this
     }
-  ⟨out, IsExtensionBy_set cache out idx hmarkbound (by simp [out])⟩
+  ⟨out, IsExtensionBy_set cache out idx .top hmarkbound (by simp [out]) (by simp)⟩
 
 /--
 Add a `Decl.atom` to a cache.
@@ -315,15 +599,15 @@ def Cache.addAtom (cache : Cache aig cnf) (idx : Nat) (h : idx < aig.decls.size)
     {
       out : Cache aig ((cnf ++ Decl.atomToCNF idx (a + aig.decls.size)))
         //
-      Cache.IsExtensionBy cache out idx h
+      Cache.IsExtensionBy cache out idx .top h
     } :=
   have hmarkbound : idx < cache.marks.size := by have := cache.hmarks; omega
   let out :=
     { cache with
-      marks := cache.marks.set idx true
+      marks := cache.marks.set idx .top
       hmarks := by simp [cache.hmarks]
       inv := by
-        intro assign heval idx hbound hmarked
+        intro assign heval idx inverted hbound hmarked
         rw [Array.getElem_set] at hmarked
         split at hmarked
         next heq =>
@@ -331,91 +615,224 @@ def Cache.addAtom (cache : Cache aig cnf) (idx : Nat) (h : idx < aig.decls.size)
           simp [heval, denote_idx_atom htip]
         next heq =>
           simp only [CNF.eval_append, Decl.atomToCNF_eval, Bool.and_eq_true, beq_iff_eq] at heval
-          have := cache.inv assign heval.left idx hbound hmarked
-          rw [this]
+          have := cache.inv assign heval.left idx inverted hbound hmarked
+          apply this
     }
-  ⟨out, IsExtensionBy_set cache out idx hmarkbound (by simp [out])⟩
+  ⟨out, IsExtensionBy_set cache out idx .top hmarkbound (by simp [out]) (by simp)⟩
 
-/--
-Add a `Decl.gate` to a cache.
--/
-def Cache.addGate (cache : Cache aig cnf) {hlb} {hrb} (idx : Nat) (h : idx < aig.decls.size)
-    (htip : aig.decls[idx]'h = .gate lhs rhs) (hl : cache.marks[lhs.gate]'hlb = true)
-    (hr : cache.marks[rhs.gate]'hrb = true) :
+def Cache.addGatePos (cache : Cache aig cnf) {hlb} {hrb} (idx : Nat) (h : idx < aig.decls.size)
+    (htip : aig.decls[idx]'h = .gate lhs rhs) (hl : cache.marks[lhs.gate]'hlb |>.has lhs.invert)
+    (hr : cache.marks[rhs.gate]'hrb |>.has rhs.invert) :
     {
-      out : Cache aig (cnf ++ Decl.gateToCNF idx lhs.gate rhs.gate lhs.invert rhs.invert)
+      out : Cache aig (cnf ++ Decl.gatePosToCNF idx lhs.gate rhs.gate lhs.invert rhs.invert)
         //
-      Cache.IsExtensionBy cache out idx h
+      Cache.IsExtensionBy cache out idx .uninverted h
     } :=
   have := aig.hdag h htip
   have hmarkbound : idx < cache.marks.size := by have := cache.hmarks; omega
   let out :=
     { cache with
-      marks := cache.marks.set idx true
+      marks := cache.marks.modify idx (·.join .uninverted)
       hmarks := by simp [cache.hmarks]
       inv := by
-        intro assign heval idx hbound hmarked
-        rw [Array.getElem_set] at hmarked
+        intro assign heval idx inverted hbound hmarked
+        rw [Array.getElem_modify] at hmarked
         split at hmarked
         next heq =>
-          simp only [heq, CNF.eval_append, Decl.gateToCNF_eval, Bool.and_eq_true, beq_iff_eq]
-            at htip heval
-          have hleval := cache.inv assign heval.left lhs.gate (by omega) hl
-          have hreval := cache.inv assign heval.left rhs.gate (by omega) hr
-          simp only [denote_idx_gate htip, Bool.bne_false, projectRightAssign_property, heval]
-          generalize lhs.invert = linv
-          generalize rhs.invert = rinv
-          cases linv <;> cases rinv <;> simp [hleval, hreval]
+          simp only [heq, CNF.eval_append, Decl.gatePosToCNF_eval, ge_iff_le, Bool.and_eq_true,
+            decide_eq_true_eq] at htip heval
+          cases inverted
+          · have hleval := cache.inv assign heval.left lhs.gate lhs.invert (by omega) hl
+            have hreval := cache.inv assign heval.left rhs.gate rhs.invert (by omega) hr
+            simp [denote_idx_gate htip]
+            replace heval := heval.right
+            revert heval hleval hreval
+            simp only [show ∀ (f : Fanin) h assign, ⟦aig, ⟨f.gate, f.invert, h⟩, assign⟧ = (⟦aig, ⟨f.gate, false, h⟩, assign⟧ ^^ f.invert) by
+              intro f; cases f.invert <;> simp, projectRightAssign_property]
+            generalize lhs.invert = linv
+            generalize rhs.invert = rinv
+            generalize ⟦aig, ⟨lhs.gate, false, by omega⟩, projectLeftAssign aig assign⟧ = lval
+            generalize ⟦aig, ⟨rhs.gate, false, by omega⟩, projectLeftAssign aig assign⟧ = rval
+            generalize assign lhs.gate = lgate
+            generalize assign rhs.gate = rgate
+            generalize assign idx = out
+            decide +revert
+          · simp at hmarked
+            apply cache.inv assign heval.left idx true hbound hmarked
         next heq =>
-          simp only [CNF.eval_append, Decl.gateToCNF_eval, Bool.and_eq_true, beq_iff_eq] at heval
-          have := cache.inv assign heval.left idx hbound hmarked
-          rw [this]
+          simp only [CNF.eval_append, Bool.and_eq_true] at heval
+          apply cache.inv assign heval.left idx inverted hbound hmarked
     }
-  ⟨out, IsExtensionBy_set cache out idx hmarkbound (by simp [out])⟩
+  ⟨out, IsExtensionBy_modify cache out idx .uninverted hmarkbound (by simp [out])⟩
 
-/--
-Add an if-then-else gate to a cache.
--/
-def Cache.addIte (cache : Cache aig cnf) {cond ifTrue ifFalse : Fanin} (idx : Nat) {hcb htb hfb}
+def Cache.addGateNeg (cache : Cache aig cnf) {hlb} {hrb} (idx : Nat) (h : idx < aig.decls.size)
+    (htip : aig.decls[idx]'h = .gate lhs rhs) (hl : cache.marks[lhs.gate]'hlb |>.has !lhs.invert)
+    (hr : cache.marks[rhs.gate]'hrb |>.has !rhs.invert) :
+    {
+      out : Cache aig (cnf ++ Decl.gateNegToCNF idx lhs.gate rhs.gate lhs.invert rhs.invert)
+        //
+      Cache.IsExtensionBy cache out idx .inverted h
+    } :=
+  have := aig.hdag h htip
+  have hmarkbound : idx < cache.marks.size := by have := cache.hmarks; omega
+  let out :=
+    { cache with
+      marks := cache.marks.modify idx (·.join .inverted)
+      hmarks := by simp [cache.hmarks]
+      inv := by
+        intro assign heval idx inverted hbound hmarked
+        rw [Array.getElem_modify] at hmarked
+        split at hmarked
+        next heq =>
+          simp only [heq, CNF.eval_append, Decl.gateNegToCNF_eval, Bool.and_eq_true,
+            decide_eq_true_eq] at htip heval
+          cases inverted
+          · simp at hmarked
+            apply cache.inv assign heval.left idx false hbound hmarked
+          · have hleval := cache.inv assign heval.left lhs.gate (!lhs.invert) (by omega) hl
+            have hreval := cache.inv assign heval.left rhs.gate (!rhs.invert) (by omega) hr
+            simp [denote_idx_gate htip]
+            replace heval := heval.right
+            revert heval hleval hreval
+            simp only [show ∀ g inv h assign, ⟦aig, ⟨g, !inv, h⟩, assign⟧ = !⟦aig, ⟨g, inv, h⟩, assign⟧ by
+              intro f inv; cases inv <;> simp, projectRightAssign_property]
+            simp only [show ∀ (f : Fanin) h assign, ⟦aig, ⟨f.gate, f.invert, h⟩, assign⟧ = (⟦aig, ⟨f.gate, false, h⟩, assign⟧ ^^ f.invert) by
+              intro f; cases f.invert <;> simp]
+            generalize lhs.invert = linv
+            generalize rhs.invert = rinv
+            generalize ⟦aig, ⟨lhs.gate, false, by omega⟩, projectLeftAssign aig assign⟧ = lval
+            generalize ⟦aig, ⟨rhs.gate, false, by omega⟩, projectLeftAssign aig assign⟧ = rval
+            generalize assign lhs.gate = lgate
+            generalize assign rhs.gate = rgate
+            generalize assign idx = out
+            decide +revert
+        next heq =>
+          simp only [CNF.eval_append, Bool.and_eq_true] at heval
+          apply cache.inv assign heval.left idx inverted hbound hmarked
+    }
+  ⟨out, IsExtensionBy_modify cache out idx .inverted hmarkbound (by simp [out])⟩
+
+def Cache.addItePos (cache : Cache aig cnf) {cond ifTrue ifFalse : Fanin} (idx : Nat) {hcb htb hfb}
     (h : idx < aig.decls.size)
     (hltc : cond.gate < idx) (hltt : ifTrue.gate < idx) (hltf : ifFalse.gate < idx)
-    (hc : cache.marks[cond.gate]'hcb = true)
-    (ht : cache.marks[ifTrue.gate]'htb = true)
-    (hf : cache.marks[ifFalse.gate]'hfb = true)
+    (hc : cache.marks[cond.gate]'hcb = .top)
+    (ht : cache.marks[ifTrue.gate]'htb |>.has ifTrue.invert)
+    (hf : cache.marks[ifFalse.gate]'hfb |>.has ifFalse.invert)
     (hdenote : ∀ assign, ⟦aig, ⟨idx, false, h⟩, assign⟧ =
       ite
         ⟦aig, ⟨cond.gate, cond.invert, by omega⟩, assign⟧
         ⟦aig, ⟨ifTrue.gate, ifTrue.invert, by omega⟩, assign⟧
         ⟦aig, ⟨ifFalse.gate, ifFalse.invert, by omega⟩, assign⟧) :
     {
-      out : Cache aig (cnf ++ Decl.iteToCNF idx cond.gate ifTrue.gate ifFalse.gate cond.invert ifTrue.invert ifFalse.invert)
+      out : Cache aig (cnf ++ Decl.itePosToCNF idx cond.gate ifTrue.gate ifFalse.gate cond.invert ifTrue.invert ifFalse.invert)
         //
-      Cache.IsExtensionBy cache out idx h
+      Cache.IsExtensionBy cache out idx .uninverted h
     } :=
   have hmarkbound : idx < cache.marks.size := by have := cache.hmarks; omega
   let out :=
     { cache with
-      marks := cache.marks.set idx true
+      marks := cache.marks.modify idx (·.join .uninverted)
       hmarks := by simp [cache.hmarks]
       inv := by
-        intro assign heval idx hbound hmarked
-        rw [Array.getElem_set] at hmarked
+        intro assign heval idx inverted hbound hmarked
+        rw [Array.getElem_modify] at hmarked
         split at hmarked
         next heq =>
-          simp only [heq, CNF.eval_append, Decl.iteToCNF_eval, Bool.and_eq_true, beq_iff_eq] at heval
-          subst heq
-          have hceval := cache.inv assign heval.left cond.gate (by omega) hc
-          have hteval := cache.inv assign heval.left ifTrue.gate (by omega) ht
-          have hfeval := cache.inv assign heval.left ifFalse.gate (by omega) hf
-          have {fi : Fanin} {aig h} {assign : Nat → Bool} :
-            ⟦aig, ⟨fi.gate, fi.invert, h⟩, assign⟧ = (⟦aig, ⟨fi.gate, false, h⟩, assign⟧ ^^ fi.invert) := by
-              cases fi.invert <;> simp
-          simp [hdenote, heval, this, hceval, hteval, hfeval]
+          simp only [CNF.eval_append, Decl.itePosToCNF_eval, ge_iff_le, Bool.and_eq_true,
+            decide_eq_true_eq] at heval
+          cases inverted
+          · have hcpeval := cache.inv assign heval.left cond.gate cond.invert (by omega) (by simp [hc])
+            have hcneval := cache.inv assign heval.left cond.gate (!cond.invert) (by omega) (by simp [hc])
+            have hteval := cache.inv assign heval.left ifTrue.gate ifTrue.invert (by omega) ht
+            have hfeval := cache.inv assign heval.left ifFalse.gate ifFalse.invert (by omega) hf
+            replace heval := heval.right
+            subst heq
+            simp only [hdenote]
+            revert heval hcpeval hcneval hteval hfeval
+            simp only [show ∀ g inv h assign, ⟦aig, ⟨g, !inv, h⟩, assign⟧ = !⟦aig, ⟨g, inv, h⟩, assign⟧ by
+              intro f inv; cases inv <;> simp, projectRightAssign_property]
+            simp only [show ∀ (f : Fanin) h assign, ⟦aig, ⟨f.gate, f.invert, h⟩, assign⟧ = (⟦aig, ⟨f.gate, false, h⟩, assign⟧ ^^ f.invert) by
+              intro f; cases f.invert <;> simp]
+            generalize cond.invert = cinv
+            generalize ifTrue.invert = tinv
+            generalize ifFalse.invert = finv
+            generalize ⟦aig, ⟨cond.gate, false, by omega⟩, projectLeftAssign aig assign⟧ = cval
+            generalize ⟦aig, ⟨ifTrue.gate, false, by omega⟩, projectLeftAssign aig assign⟧ = tval
+            generalize ⟦aig, ⟨ifFalse.gate, false, by omega⟩, projectLeftAssign aig assign⟧ = fval
+            generalize assign cond.gate = cgate
+            generalize assign ifTrue.gate = tgate
+            generalize assign ifFalse.gate = fgate
+            generalize assign idx = out
+            decide +revert
+          · simp at hmarked
+            apply cache.inv assign heval.left idx true hbound hmarked
         next heq =>
-          simp only [CNF.eval_append, Decl.iteToCNF_eval, Bool.and_eq_true, beq_iff_eq] at heval
-          rw [cache.inv assign heval.left idx hbound hmarked]
+          simp only [CNF.eval_append, Bool.and_eq_true] at heval
+          apply cache.inv assign heval.left idx inverted hbound hmarked
     }
-  ⟨out, IsExtensionBy_set cache out idx hmarkbound (by simp [out])⟩
+  ⟨out, IsExtensionBy_modify cache out idx .uninverted hmarkbound (by simp [out])⟩
+
+def Cache.addIteNeg (cache : Cache aig cnf) {cond ifTrue ifFalse : Fanin} (idx : Nat) {hcb htb hfb}
+    (h : idx < aig.decls.size)
+    (hltc : cond.gate < idx) (hltt : ifTrue.gate < idx) (hltf : ifFalse.gate < idx)
+    (hc : cache.marks[cond.gate]'hcb = .top)
+    (ht : cache.marks[ifTrue.gate]'htb |>.has !ifTrue.invert)
+    (hf : cache.marks[ifFalse.gate]'hfb |>.has !ifFalse.invert)
+    (hdenote : ∀ assign, ⟦aig, ⟨idx, false, h⟩, assign⟧ =
+      ite
+        ⟦aig, ⟨cond.gate, cond.invert, by omega⟩, assign⟧
+        ⟦aig, ⟨ifTrue.gate, ifTrue.invert, by omega⟩, assign⟧
+        ⟦aig, ⟨ifFalse.gate, ifFalse.invert, by omega⟩, assign⟧) :
+    {
+      out : Cache aig (cnf ++ Decl.iteNegToCNF idx cond.gate ifTrue.gate ifFalse.gate cond.invert ifTrue.invert ifFalse.invert)
+        //
+      Cache.IsExtensionBy cache out idx .inverted h
+    } :=
+  have hmarkbound : idx < cache.marks.size := by have := cache.hmarks; omega
+  let out :=
+    { cache with
+      marks := cache.marks.modify idx (·.join .inverted)
+      hmarks := by simp [cache.hmarks]
+      inv := by
+        intro assign heval idx inverted hbound hmarked
+        rw [Array.getElem_modify] at hmarked
+        split at hmarked
+        next heq =>
+          simp only [CNF.eval_append, Decl.iteNegToCNF_eval, Bool.and_eq_true,
+            decide_eq_true_eq] at heval
+          cases inverted
+          · simp at hmarked
+            apply cache.inv assign heval.left idx false hbound hmarked
+          · have hcpeval := cache.inv assign heval.left cond.gate cond.invert (by omega) (by simp [hc])
+            have hcneval := cache.inv assign heval.left cond.gate (!cond.invert) (by omega) (by simp [hc])
+            have hteval := cache.inv assign heval.left ifTrue.gate (!ifTrue.invert) (by omega) ht
+            have hfeval := cache.inv assign heval.left ifFalse.gate (!ifFalse.invert) (by omega) hf
+            replace heval := heval.right
+            subst heq
+            rw [show ∀ g inv h assign, ⟦aig, ⟨g, inv, h⟩, assign⟧ = (⟦aig, ⟨g, false, h⟩, assign⟧ ^^ inv) by
+              intro f inv; cases inv <;> simp, projectRightAssign_property]
+            simp only [hdenote]
+            revert heval hcpeval hcneval hteval hfeval
+            simp only [show ∀ g inv h assign, ⟦aig, ⟨g, !inv, h⟩, assign⟧ = !⟦aig, ⟨g, inv, h⟩, assign⟧ by
+              intro f inv; cases inv <;> simp, projectRightAssign_property]
+            simp only [show ∀ (f : Fanin) h assign, ⟦aig, ⟨f.gate, f.invert, h⟩, assign⟧ = (⟦aig, ⟨f.gate, false, h⟩, assign⟧ ^^ f.invert) by
+              intro f; cases f.invert <;> simp]
+            generalize cond.invert = cinv
+            generalize ifTrue.invert = tinv
+            generalize ifFalse.invert = finv
+            generalize ⟦aig, ⟨cond.gate, false, by omega⟩, projectLeftAssign aig assign⟧ = cval
+            generalize ⟦aig, ⟨ifTrue.gate, false, by omega⟩, projectLeftAssign aig assign⟧ = tval
+            generalize ⟦aig, ⟨ifFalse.gate, false, by omega⟩, projectLeftAssign aig assign⟧ = fval
+            generalize assign cond.gate = cgate
+            generalize assign ifTrue.gate = tgate
+            generalize assign ifFalse.gate = fgate
+            generalize assign idx = out
+            decide +revert
+        next heq =>
+          simp only [CNF.eval_append, Bool.and_eq_true] at heval
+          apply cache.inv assign heval.left idx inverted hbound hmarked
+    }
+  ⟨out, IsExtensionBy_modify cache out idx .inverted hmarkbound (by simp [out])⟩
 
 /--
 The key invariant about the `State` itself (without cache): The CNF we produce is always satisfiable
@@ -459,12 +876,9 @@ theorem State.Inv_atomToCNF {h : upper < aig.decls.size}
   intro assign1
   simp [CNF.sat_def, denote_idx_atom heq, h]
 
-/--
-`State.Inv` holds for the CNF that we produce for a `Decl.gate`
--/
-theorem State.Inv_gateToCNF {aig : AIG Nat} {h}
+theorem State.Inv_gatePosToCNF {aig : AIG Nat} {h}
     (heq : aig.decls[upper]'h = .gate lhs rhs) :
-    State.Inv aig (Decl.gateToCNF upper lhs.gate rhs.gate lhs.invert rhs.invert) := by
+    State.Inv aig (Decl.gatePosToCNF upper lhs.gate rhs.gate lhs.invert rhs.invert) := by
   intro assign1
   have hlhs : lhs.gate < aig.decls.size := Nat.lt_trans (aig.hdag h heq).left h
   have hrhs : rhs.gate < aig.decls.size := Nat.lt_trans (aig.hdag h heq).right h
@@ -473,10 +887,18 @@ theorem State.Inv_gateToCNF {aig : AIG Nat} {h}
   rw [CNF.sat_def]
   cases linv <;> cases rinv <;> simp [denote_idx_gate heq, hlinv, hrinv, h, hlhs, hrhs]
 
-/--
-`State.Inv` holds for the CNF that we produce for an ITE.
--/
-theorem State.Inv_iteToCNF {aig : AIG Nat} {cond ifTrue ifFalse : Fanin} {idx : Nat}
+theorem State.Inv_gateNegToCNF {aig : AIG Nat} {h}
+    (heq : aig.decls[upper]'h = .gate lhs rhs) :
+    State.Inv aig (Decl.gateNegToCNF upper lhs.gate rhs.gate lhs.invert rhs.invert) := by
+  intro assign1
+  have hlhs : lhs.gate < aig.decls.size := Nat.lt_trans (aig.hdag h heq).left h
+  have hrhs : rhs.gate < aig.decls.size := Nat.lt_trans (aig.hdag h heq).right h
+  generalize hlinv : lhs.invert = linv
+  generalize hrinv : rhs.invert = rinv
+  rw [CNF.sat_def]
+  cases linv <;> cases rinv <;> simp [denote_idx_gate heq, hlinv, hrinv, h, hlhs, hrhs]
+
+theorem State.Inv_itePosToCNF {aig : AIG Nat} {cond ifTrue ifFalse : Fanin} {idx : Nat}
     (h : idx < aig.decls.size)
     (hltc : cond.gate < idx) (hltt : ifTrue.gate < idx) (hltf : ifFalse.gate < idx)
     (hdenote : ∀ assign, ⟦aig, ⟨idx, false, h⟩, assign⟧ =
@@ -484,9 +906,26 @@ theorem State.Inv_iteToCNF {aig : AIG Nat} {cond ifTrue ifFalse : Fanin} {idx : 
         ⟦aig, ⟨cond.gate, cond.invert, by omega⟩, assign⟧
         ⟦aig, ⟨ifTrue.gate, ifTrue.invert, by omega⟩, assign⟧
         ⟦aig, ⟨ifFalse.gate, ifFalse.invert, by omega⟩, assign⟧) :
-    State.Inv aig (Decl.iteToCNF idx cond.gate ifTrue.gate ifFalse.gate cond.invert ifTrue.invert ifFalse.invert) := by
+    State.Inv aig (Decl.itePosToCNF idx cond.gate ifTrue.gate ifFalse.gate cond.invert ifTrue.invert ifFalse.invert) := by
   intro assign1
-  rw [CNF.sat_def, Decl.iteToCNF_eval, satAssignment_inr h, hdenote, satAssignment_inr (by omega),
+  rw [CNF.sat_def, Decl.itePosToCNF_eval, satAssignment_inr h, hdenote, satAssignment_inr (by omega),
+    satAssignment_inr (by omega), satAssignment_inr (by omega)]
+  have {fi : Fanin} {aig h} {assign : Nat → Bool} :
+    ⟦aig, ⟨fi.gate, fi.invert, h⟩, assign⟧ = (⟦aig, ⟨fi.gate, false, h⟩, assign⟧ ^^ fi.invert) := by
+      cases fi.invert <;> simp
+  simp [this]
+
+theorem State.Inv_iteNegToCNF {aig : AIG Nat} {cond ifTrue ifFalse : Fanin} {idx : Nat}
+    (h : idx < aig.decls.size)
+    (hltc : cond.gate < idx) (hltt : ifTrue.gate < idx) (hltf : ifFalse.gate < idx)
+    (hdenote : ∀ assign, ⟦aig, ⟨idx, false, h⟩, assign⟧ =
+      ite
+        ⟦aig, ⟨cond.gate, cond.invert, by omega⟩, assign⟧
+        ⟦aig, ⟨ifTrue.gate, ifTrue.invert, by omega⟩, assign⟧
+        ⟦aig, ⟨ifFalse.gate, ifFalse.invert, by omega⟩, assign⟧) :
+    State.Inv aig (Decl.iteNegToCNF idx cond.gate ifTrue.gate ifFalse.gate cond.invert ifTrue.invert ifFalse.invert) := by
+  intro assign1
+  rw [CNF.sat_def, Decl.iteNegToCNF_eval, satAssignment_inr h, hdenote, satAssignment_inr (by omega),
     satAssignment_inr (by omega), satAssignment_inr (by omega)]
   have {fi : Fanin} {aig h} {assign : Nat → Bool} :
     ⟦aig, ⟨fi.gate, fi.invert, h⟩, assign⟧ = (⟦aig, ⟨fi.gate, false, h⟩, assign⟧ ^^ fi.invert) := by
@@ -521,20 +960,20 @@ def State.empty (aig : AIG Nat) : State aig where
 /--
 State extension are `Cache.IsExtensionBy` for now.
 -/
-abbrev State.IsExtensionBy (state1 : State aig) (state2 : State aig) (new : Nat)
+abbrev State.IsExtensionBy (state1 : State aig) (state2 : State aig) (new : Nat) (mark : BiMark)
     (hnew : new < aig.decls.size) : Prop :=
-  Cache.IsExtensionBy state1.cache state2.cache new hnew
+  Cache.IsExtensionBy state1.cache state2.cache new mark hnew
 
 theorem State.IsExtensionBy_trans_left (state1 : State aig) (state2 : State aig)
-    (state3 : State aig) (h12 : IsExtensionBy state1 state2 new1 hnew1)
-    (h23 : IsExtensionBy state2 state3 new2 hnew2) : IsExtensionBy state1 state3 new1 hnew1 := by
-  apply  Cache.IsExtensionBy_trans_left
+    (state3 : State aig) (h12 : IsExtensionBy state1 state2 new1 mark1 hnew1)
+    (h23 : IsExtensionBy state2 state3 new2 mark2 hnew2) : IsExtensionBy state1 state3 new1 mark1 hnew1 := by
+  apply Cache.IsExtensionBy_trans_left
   · exact h12
   · exact h23
 
 theorem State.IsExtensionBy_trans_right (state1 : State aig) (state2 : State aig)
-    (state3 : State aig) (h12 : IsExtensionBy state1 state2 new1 hnew1)
-    (h23 : IsExtensionBy state2 state3 new2 hnew2) : IsExtensionBy state1 state3 new2 hnew2 := by
+    (state3 : State aig) (h12 : IsExtensionBy state1 state2 new1 mark1 hnew1)
+    (h23 : IsExtensionBy state2 state3 new2 mark2 hnew2) : IsExtensionBy state1 state3 new2 mark2 hnew2 := by
   apply  Cache.IsExtensionBy_trans_right
   · exact h12
   · exact h23
@@ -543,16 +982,28 @@ theorem State.IsExtensionBy_trans_right (state1 : State aig) (state2 : State aig
 State extension is a reflexive relation.
 -/
 theorem State.IsExtensionBy_rfl (state : State aig) {h}
-    (hmarked : state.cache.marks[idx]'h = true) :
-    State.IsExtensionBy state state idx (have := state.cache.hmarks; omega) := by
+    (hmarked : mark ≤ state.cache.marks[idx]'h) :
+    State.IsExtensionBy state state idx mark (have := state.cache.hmarks; omega) := by
   apply Cache.IsExtensionBy_rfl <;> assumption
+
+theorem State.IsExtensionBy_le {state1 : State aig} {state2 : State aig} {h}
+    (h12 : IsExtensionBy state1 state2 idx mark1 h) (hle : mark2 ≤ mark1) :
+    IsExtensionBy state1 state2 idx mark2 hnew := by
+  apply Cache.IsExtensionBy_le <;> assumption
+
+theorem State.IsExtensionBy_join {state1 : State aig} {state2 : State aig} {h}
+    (h1 : State.IsExtensionBy state1 state2 idx mark1 h)
+    (h2 : State.IsExtensionBy state1 state2 idx mark2 h)
+    (hjoin : mark3 ≤ mark1.join mark2) :
+    State.IsExtensionBy state1 state2 idx mark3 hnew := by
+  exact Cache.IsExtensionBy_join h1 h2 hjoin
 
 /--
 Add the CNF for a `Decl.false` to the state.
 -/
 def State.addFalse (state : State aig) (idx : Nat) (h : idx < aig.decls.size)
     (htip : aig.decls[idx]'h = .false) :
-    { out : State aig // State.IsExtensionBy state out idx h } :=
+    { out : State aig // State.IsExtensionBy state out idx .top h } :=
   let ⟨cnf, cache, inv⟩ := state
   let newCnf := Decl.falseToCNF idx
   have hinv := toCNF.State.Inv_falseToCNF htip
@@ -564,46 +1015,69 @@ Add the CNF for a `Decl.atom` to the state.
 -/
 def State.addAtom (state : State aig) (idx : Nat) (h : idx < aig.decls.size)
     (htip : aig.decls[idx]'h = .atom a) :
-    { out : State aig // State.IsExtensionBy state out idx h } :=
+    { out : State aig // State.IsExtensionBy state out idx .top h } :=
   let ⟨cnf, cache, inv⟩ := state
   let newCnf := Decl.atomToCNF idx (a + aig.decls.size)
   have hinv := toCNF.State.Inv_atomToCNF htip
   let ⟨cache, hcache⟩ := cache.addAtom idx h htip
   ⟨⟨cnf ++ newCnf, cache, State.Inv_append inv hinv⟩, by simp [newCnf, hcache]⟩
 
-/--
-Add the CNF for a `Decl.gate` to the state.
--/
-def State.addGate (state : State aig) {hlb} {hrb} (idx : Nat) (h : idx < aig.decls.size)
-    (htip : aig.decls[idx]'h = .gate lhs rhs) (hl : state.cache.marks[lhs.gate]'hlb = true)
-    (hr : state.cache.marks[rhs.gate]'hrb = true) :
-    { out : State aig // State.IsExtensionBy state out idx h } :=
+def State.addGatePos (state : State aig) {hlb} {hrb} (idx : Nat) (h : idx < aig.decls.size)
+    (htip : aig.decls[idx]'h = .gate lhs rhs) (hl : state.cache.marks[lhs.gate]'hlb |>.has lhs.invert)
+    (hr : state.cache.marks[rhs.gate]'hrb |>.has rhs.invert ) :
+    { out : State aig // State.IsExtensionBy state out idx .uninverted h } :=
   have := aig.hdag h htip
   let ⟨cnf, cache, inv⟩ := state
-  let newCnf := Decl.gateToCNF idx lhs.gate rhs.gate lhs.invert rhs.invert
-  have hinv := toCNF.State.Inv_gateToCNF htip
-  let ⟨cache, hcache⟩ := cache.addGate idx h htip hl hr
+  let newCnf := Decl.gatePosToCNF idx lhs.gate rhs.gate lhs.invert rhs.invert
+  have hinv := toCNF.State.Inv_gatePosToCNF htip
+  let ⟨cache, hcache⟩ := cache.addGatePos idx h htip hl hr
   ⟨⟨cnf ++ newCnf, cache, State.Inv_append inv hinv⟩, by simp [newCnf, hcache]⟩
 
-/--
-Add the CNF for an if-then-else to the state.
--/
-def State.addIte (state : State aig) {cond ifTrue ifFalse : Fanin} (idx : Nat) {hcb htb hfb}
+def State.addGateNeg (state : State aig) {hlb} {hrb} (idx : Nat) (h : idx < aig.decls.size)
+    (htip : aig.decls[idx]'h = .gate lhs rhs) (hl : state.cache.marks[lhs.gate]'hlb |>.has !lhs.invert)
+    (hr : state.cache.marks[rhs.gate]'hrb |>.has !rhs.invert ) :
+    { out : State aig // State.IsExtensionBy state out idx .inverted h } :=
+  have := aig.hdag h htip
+  let ⟨cnf, cache, inv⟩ := state
+  let newCnf := Decl.gateNegToCNF idx lhs.gate rhs.gate lhs.invert rhs.invert
+  have hinv := toCNF.State.Inv_gateNegToCNF htip
+  let ⟨cache, hcache⟩ := cache.addGateNeg idx h htip hl hr
+  ⟨⟨cnf ++ newCnf, cache, State.Inv_append inv hinv⟩, by simp [newCnf, hcache]⟩
+
+def State.addItePos (state : State aig) {cond ifTrue ifFalse : Fanin} (idx : Nat) {hcb htb hfb}
     (h : idx < aig.decls.size)
     (hltc : cond.gate < idx) (hltt : ifTrue.gate < idx) (hltf : ifFalse.gate < idx)
-    (hc : state.cache.marks[cond.gate]'hcb = true)
-    (ht : state.cache.marks[ifTrue.gate]'htb = true)
-    (hf : state.cache.marks[ifFalse.gate]'hfb = true)
+    (hc : state.cache.marks[cond.gate]'hcb = .top)
+    (ht : state.cache.marks[ifTrue.gate]'htb |>.has ifTrue.invert)
+    (hf : state.cache.marks[ifFalse.gate]'hfb |>.has ifFalse.invert)
     (hdenote : ∀ assign, ⟦aig, ⟨idx, false, h⟩, assign⟧ =
       ite
         ⟦aig, ⟨cond.gate, cond.invert, by omega⟩, assign⟧
         ⟦aig, ⟨ifTrue.gate, ifTrue.invert, by omega⟩, assign⟧
         ⟦aig, ⟨ifFalse.gate, ifFalse.invert, by omega⟩, assign⟧) :
-    { out : State aig // State.IsExtensionBy state out idx h } :=
+    { out : State aig // State.IsExtensionBy state out idx .uninverted h } :=
   let ⟨cnf, cache, inv⟩ := state
-  let newCnf := Decl.iteToCNF idx cond.gate ifTrue.gate ifFalse.gate cond.invert ifTrue.invert ifFalse.invert
-  have hinv := toCNF.State.Inv_iteToCNF h hltc hltt hltf hdenote
-  let ⟨cache, hcache⟩ := cache.addIte idx h hltc hltt hltf hc ht hf hdenote
+  let newCnf := Decl.itePosToCNF idx cond.gate ifTrue.gate ifFalse.gate cond.invert ifTrue.invert ifFalse.invert
+  have hinv := toCNF.State.Inv_itePosToCNF h hltc hltt hltf hdenote
+  let ⟨cache, hcache⟩ := cache.addItePos idx h hltc hltt hltf hc ht hf hdenote
+  ⟨⟨cnf ++ newCnf, cache, State.Inv_append inv hinv⟩, by simp [newCnf, hcache]⟩
+
+def State.addIteNeg (state : State aig) {cond ifTrue ifFalse : Fanin} (idx : Nat) {hcb htb hfb}
+    (h : idx < aig.decls.size)
+    (hltc : cond.gate < idx) (hltt : ifTrue.gate < idx) (hltf : ifFalse.gate < idx)
+    (hc : state.cache.marks[cond.gate]'hcb = .top)
+    (ht : state.cache.marks[ifTrue.gate]'htb |>.has !ifTrue.invert)
+    (hf : state.cache.marks[ifFalse.gate]'hfb |>.has !ifFalse.invert)
+    (hdenote : ∀ assign, ⟦aig, ⟨idx, false, h⟩, assign⟧ =
+      ite
+        ⟦aig, ⟨cond.gate, cond.invert, by omega⟩, assign⟧
+        ⟦aig, ⟨ifTrue.gate, ifTrue.invert, by omega⟩, assign⟧
+        ⟦aig, ⟨ifFalse.gate, ifFalse.invert, by omega⟩, assign⟧) :
+    { out : State aig // State.IsExtensionBy state out idx .inverted h } :=
+  let ⟨cnf, cache, inv⟩ := state
+  let newCnf := Decl.iteNegToCNF idx cond.gate ifTrue.gate ifFalse.gate cond.invert ifTrue.invert ifFalse.invert
+  have hinv := toCNF.State.Inv_iteNegToCNF h hltc hltt hltf hdenote
+  let ⟨cache, hcache⟩ := cache.addIteNeg idx h hltc hltt hltf hc ht hf hdenote
   ⟨⟨cnf ++ newCnf, cache, State.Inv_append inv hinv⟩, by simp [newCnf, hcache]⟩
 
 /--
@@ -780,61 +1254,178 @@ end toCNF
 Convert an AIG into CNF, starting at some entry node.
 -/
 public def toCNF (entry : Entrypoint Nat) : CNF Nat :=
-  let ⟨state, _⟩ := go entry.aig entry.ref.gate entry.ref.hgate (toCNF.State.empty entry.aig)
+  let ⟨state, _⟩ := go entry.aig entry.ref.gate (.of entry.ref.invert) entry.ref.hgate (toCNF.State.empty entry.aig)
   state.cnf.add (CNF.Clause.empty.add entry.ref.gate !entry.ref.invert)
 where
-  go (aig : AIG Nat) (upper : Nat) (h : upper < aig.decls.size) (state : toCNF.State aig) :
-      { out : toCNF.State aig // toCNF.State.IsExtensionBy state out upper h } :=
-    if hmarked : state.cache.marks[upper]'(by have := state.cache.hmarks; omega) then
+  go (aig : AIG Nat) (upper : Nat) (mark : toCNF.BiMark) (h : upper < aig.decls.size) (state : toCNF.State aig) :
+      { out : toCNF.State aig // toCNF.State.IsExtensionBy state out upper mark h } :=
+    let existingMark := state.cache.marks[upper]'(by have := state.cache.hmarks; omega)
+    if hmarked : mark ≤ existingMark then
       ⟨state, by apply toCNF.State.IsExtensionBy_rfl <;> assumption⟩
     else
       let decl := aig.decls[upper]
       match heq : decl with
-      | .false => state.addFalse upper h heq
-      | .atom _ => state.addAtom upper h heq
+      | .false =>
+        let res := state.addFalse upper h heq
+        ⟨res.val, toCNF.State.IsExtensionBy_le res.property (by simp)⟩
+      | .atom _ =>
+        let res := state.addAtom upper h heq
+        ⟨res.val, toCNF.State.IsExtensionBy_le res.property (by simp)⟩
       | .gate lhs rhs =>
+        -- Only add the marks not present in the existing mark
+        let fullMark := mark
+        let mark := mark.sub existingMark
+        have hmarkmeet {other} :
+            state.IsExtensionBy other upper mark (by omega) →
+            state.IsExtensionBy other upper fullMark (by omega) := by
+          intro h
+          have : state.IsExtensionBy other upper existingMark (by omega) := by
+            apply toCNF.State.IsExtensionBy_trans_left (h23 := h)
+            subst existingMark
+            apply toCNF.State.IsExtensionBy_rfl
+            · assumption
+            · simp
+            · have := state.cache.hmarks; omega
+          apply toCNF.Cache.IsExtensionBy_join h this
+          simp [mark, fullMark]
+
         match hite : toCNF.detectIte upper h with
         | some ⟨cond, ifTrue, ifFalse⟩ =>
           have hltc := toCNF.detectIte_cond_lt hite
           have hltt := toCNF.detectIte_ifTrue_lt hite
           have hltf := toCNF.detectIte_ifFalse_lt hite
 
-          let ⟨cstate, hcstate⟩ := go aig cond.gate (by omega) state
-          let ⟨tstate, htstate⟩ := go aig ifTrue.gate (by omega) cstate
-          let ⟨fstate, hfstate⟩ := go aig ifFalse.gate (by omega) tstate
+          let ⟨cstate, hcstate⟩ := go aig cond.gate .top (by omega) state
+          let ⟨tstate, htstate⟩ := go aig ifTrue.gate (mark.invert ifTrue.invert) (by omega) cstate
+          let ⟨fstate, hfstate⟩ := go aig ifFalse.gate (mark.invert ifFalse.invert) (by omega) tstate
 
-          have hcstate' : toCNF.State.IsExtensionBy state fstate cond.gate (by omega) := by
+          have hcstate' : state.IsExtensionBy fstate cond.gate .top (by omega) := by
             apply toCNF.State.IsExtensionBy_trans_left (h23 := hfstate)
             apply toCNF.State.IsExtensionBy_trans_left (h23 := htstate)
             exact hcstate
 
-          have htstate' : toCNF.State.IsExtensionBy cstate fstate ifTrue.gate (by omega) := by
+          have htstate' : cstate.IsExtensionBy fstate ifTrue.gate (mark.invert ifTrue.invert) (by omega) := by
             apply toCNF.State.IsExtensionBy_trans_left (h23 := hfstate)
             exact htstate
 
-          let ⟨ret, hretstate⟩ := fstate.addIte upper h hltc hltt hltf hcstate'.trueAt htstate'.trueAt hfstate.trueAt
-            (by simp [toCNF.denote_detectIte hite])
-          ⟨ret, toCNF.State.IsExtensionBy_trans_right (h12 := hcstate') (h23 := hretstate)⟩
+          let ⟨posstate, hposstate⟩ : { out // fstate.IsExtensionBy out upper (mark.meet .uninverted) h } :=
+            if hmark : mark.has false then
+              let res :=
+                fstate.addItePos upper h hltc hltt hltf
+                  (toCNF.BiMark.top_le.mp hcstate'.trueAt)
+                  (by apply toCNF.BiMark.has_of_le htstate'.trueAt; simp [hmark])
+                  (by apply toCNF.BiMark.has_of_le hfstate.trueAt; simp [hmark])
+                  (by simp [toCNF.denote_detectIte hite])
+              ⟨res.val, toCNF.State.IsExtensionBy_le res.property (by simp)⟩
+            else
+              ⟨fstate, by
+                apply toCNF.State.IsExtensionBy_rfl
+                · assumption
+                · simp at hmark
+                  simp [toCNF.BiMark.le_iff, hmark]
+                · simpa [fstate.cache.hmarks]
+              ⟩
+
+          have hcstate'' : state.IsExtensionBy posstate cond.gate .top (by omega) := by
+            apply toCNF.State.IsExtensionBy_trans_left (h23 := hposstate)
+            · exact hcstate'
+
+          have htstate'' : cstate.IsExtensionBy posstate ifTrue.gate (mark.invert ifTrue.invert) (by omega) := by
+            apply toCNF.State.IsExtensionBy_trans_left (h23 := hposstate)
+            · exact htstate'
+
+          have hfstate'' : tstate.IsExtensionBy posstate ifFalse.gate (mark.invert ifFalse.invert) (by omega) := by
+            apply toCNF.State.IsExtensionBy_trans_left (h23 := hposstate)
+            · exact hfstate
+
+          let ⟨negstate, hnegstate⟩ : { out // posstate.IsExtensionBy out upper (mark.meet .inverted) h } :=
+            if hmark : mark.has true then
+              let res :=
+                posstate.addIteNeg upper h hltc hltt hltf
+                  (toCNF.BiMark.top_le.mp hcstate''.trueAt)
+                  (by apply toCNF.BiMark.has_of_le htstate''.trueAt; simp [hmark])
+                  (by apply toCNF.BiMark.has_of_le hfstate''.trueAt; simp [hmark])
+                  (by simp [toCNF.denote_detectIte hite])
+              ⟨res.val, toCNF.State.IsExtensionBy_le res.property (by simp)⟩
+            else
+              ⟨posstate, by
+                apply toCNF.State.IsExtensionBy_rfl
+                · assumption
+                · simp at hmark
+                  simp [toCNF.BiMark.le_iff, hmark]
+                · simpa [posstate.cache.hmarks]
+              ⟩
+
+          have hposstate' : fstate.IsExtensionBy negstate upper (mark.meet .uninverted) (by omega) := by
+            apply toCNF.State.IsExtensionBy_trans_left (h23 := hnegstate)
+            · exact hposstate
+
+          have hmarkstate : fstate.IsExtensionBy negstate upper mark (by omega) := by
+            rw [show mark = (mark.meet .uninverted).join (mark.meet .inverted) by simp [toCNF.BiMark.ext_iff]]
+            apply toCNF.State.IsExtensionBy_join hposstate' ?_ (toCNF.BiMark.le_rfl)
+            apply toCNF.State.IsExtensionBy_trans_right (h12 := hposstate) (h23 := hnegstate)
+
+          ⟨negstate, hmarkmeet <| toCNF.State.IsExtensionBy_trans_right (h12 := hcstate') (h23 := hmarkstate)⟩
         | none =>
           have := aig.hdag h heq
-          let ⟨lstate, hlstate⟩ := go aig lhs.gate (by omega) state
-          let ⟨rstate, hrstate⟩ := go aig rhs.gate (by omega) lstate
+          let ⟨lstate, hlstate⟩ := go aig lhs.gate (mark.invert lhs.invert) (by omega) state
+          let ⟨rstate, hrstate⟩ := go aig rhs.gate (mark.invert rhs.invert) (by omega) lstate
 
-          have : toCNF.State.IsExtensionBy state rstate lhs.gate (by omega) := by
+          have hlstate' : state.IsExtensionBy rstate lhs.gate (mark.invert lhs.invert) (by omega) := by
             apply toCNF.State.IsExtensionBy_trans_left
             · exact hlstate
             · exact hrstate
 
-          let ⟨ret, hretstate⟩ := rstate.addGate upper h heq this.trueAt hrstate.trueAt
-          ⟨
-            ret,
-            by
-              apply toCNF.State.IsExtensionBy_trans_right
-              · exact hlstate
-              · apply toCNF.State.IsExtensionBy_trans_right
-                · exact hrstate
-                · exact hretstate
-          ⟩
+          let ⟨posstate, hposstate⟩ : { out // rstate.IsExtensionBy out upper (mark.meet .uninverted) h } :=
+            if hmark : mark.has false then
+              let res :=
+                rstate.addGatePos upper h heq
+                  (by apply toCNF.BiMark.has_of_le hlstate'.trueAt; simp [hmark])
+                  (by apply toCNF.BiMark.has_of_le hrstate.trueAt; simp [hmark])
+              ⟨res.val, toCNF.State.IsExtensionBy_le res.property (by simp)⟩
+            else
+              ⟨rstate, by
+                apply toCNF.State.IsExtensionBy_rfl
+                · assumption
+                · simp at hmark
+                  simp [toCNF.BiMark.le_iff, hmark]
+                · simpa [rstate.cache.hmarks]
+              ⟩
+
+          have hlstate'' : state.IsExtensionBy posstate lhs.gate (mark.invert lhs.invert) (by omega) := by
+            apply toCNF.State.IsExtensionBy_trans_left (h23 := hposstate)
+            · exact hlstate'
+
+          have hrstate'' : lstate.IsExtensionBy posstate rhs.gate (mark.invert rhs.invert) (by omega) := by
+            apply toCNF.State.IsExtensionBy_trans_left (h23 := hposstate)
+            · exact hrstate
+
+          let ⟨negstate, hnegstate⟩ : { out // posstate.IsExtensionBy out upper (mark.meet .inverted) h } :=
+            if hmark : mark.has true then
+              let res :=
+                posstate.addGateNeg upper h heq
+                  (by apply toCNF.BiMark.has_of_le hlstate''.trueAt; simp [hmark])
+                  (by apply toCNF.BiMark.has_of_le hrstate''.trueAt; simp [hmark])
+              ⟨res.val, toCNF.State.IsExtensionBy_le res.property (by simp)⟩
+            else
+              ⟨posstate, by
+                apply toCNF.State.IsExtensionBy_rfl
+                · assumption
+                · simp at hmark
+                  simp [toCNF.BiMark.le_iff, hmark]
+                · simpa [posstate.cache.hmarks]
+              ⟩
+
+            have hposstate' : rstate.IsExtensionBy negstate upper (mark.meet .uninverted) (by omega) := by
+              apply toCNF.State.IsExtensionBy_trans_left (h23 := hnegstate)
+              · exact hposstate
+
+            have hmarkstate : rstate.IsExtensionBy negstate upper mark (by omega) := by
+              rw [show mark = (mark.meet .uninverted).join (mark.meet .inverted) by simp [toCNF.BiMark.ext_iff]]
+              apply toCNF.State.IsExtensionBy_join hposstate' ?_ (toCNF.BiMark.le_rfl)
+              apply toCNF.State.IsExtensionBy_trans_right (h12 := hposstate) (h23 := hnegstate)
+
+            ⟨negstate, hmarkmeet <| toCNF.State.IsExtensionBy_trans_right (h12 := hlstate') (h23 := hmarkstate)⟩
   termination_by upper
   decreasing_by all_goals omega
 
@@ -842,34 +1433,34 @@ where
 The node that we started CNF conversion at will always be marked as visited in the CNF cache.
 -/
 theorem toCNF.go_marks :
-    (go aig start h state).val.cache.marks[start]'(by have := (go aig start h state).val.cache.hmarks; omega) = true :=
-  (go aig start h state).property.trueAt
+    mark ≤ (go aig start mark h state).val.cache.marks[start]'(by have := (go aig start mark h state).val.cache.hmarks; omega) :=
+  (go aig start mark h state).property.trueAt
 
 /--
 The CNF returned by `go` will always be SAT at `cnfSatAssignment`.
 -/
-theorem toCNF.go_sat (aig : AIG Nat) (start : Nat) (h1 : start < aig.decls.size) (assign1 : Nat → Bool)
+theorem toCNF.go_sat (aig : AIG Nat) (start : Nat) (mark : BiMark) (h1 : start < aig.decls.size) (assign1 : Nat → Bool)
     (state : toCNF.State aig) :
-    (go aig start h1 state).val.Sat (cnfSatAssignment aig assign1)  := by
-  have := (go aig start h1 state).val.inv assign1
+    (go aig start mark h1 state).val.Sat (cnfSatAssignment aig assign1)  := by
+  have := (go aig start mark h1 state).val.inv assign1
   rw [State.sat_iff]
   simp [this]
 
-theorem toCNF.go_as_denote' (aig : AIG Nat) (start) (inv) (h1) (assign1) :
-    ⟦aig, ⟨start, inv, h1⟩, assign1⟧ → (go aig start h1 (.empty aig)).val.eval (cnfSatAssignment aig assign1) := by
-  have := go_sat aig start h1 assign1 (.empty aig)
+theorem toCNF.go_as_denote' (aig : AIG Nat) (start) (mark) (inv) (h1) (assign1) :
+    ⟦aig, ⟨start, inv, h1⟩, assign1⟧ → (go aig start mark h1 (.empty aig)).val.eval (cnfSatAssignment aig assign1) := by
+  have := go_sat aig start mark h1 assign1 (.empty aig)
   simp only [State.Sat, CNF.sat_def] at this
   simp [this]
 
 /--
 Connect SAT results about the CNF to SAT results about the AIG.
 -/
-theorem toCNF.go_as_denote (aig : AIG Nat) (start) (h1) (assign1) :
-    ((⟦aig, ⟨start, inv, h1⟩, assign1⟧ && (go aig start h1 (.empty aig)).val.eval (cnfSatAssignment aig assign1)) = sat?)
+theorem toCNF.go_as_denote (aig : AIG Nat) (start) (mark) (h1) (assign1) :
+    ((⟦aig, ⟨start, inv, h1⟩, assign1⟧ && (go aig start mark h1 (.empty aig)).val.eval (cnfSatAssignment aig assign1)) = sat?)
       →
     (⟦aig, ⟨start, inv, h1⟩, assign1⟧ = sat?) := by
-  have := go_as_denote' aig start inv h1 assign1
-  by_cases CNF.eval (cnfSatAssignment aig assign1) (go aig start h1 (State.empty aig)).val.cnf <;> simp_all
+  have := go_as_denote' aig start mark inv h1 assign1
+  by_cases CNF.eval (cnfSatAssignment aig assign1) (go aig start mark h1 (State.empty aig)).val.cnf <;> simp_all
 
 /--
 Connect SAT results about the AIG to SAT results about the CNF.
@@ -877,13 +1468,15 @@ Connect SAT results about the AIG to SAT results about the CNF.
 theorem toCNF.denote_as_go {assign : Nat → Bool} :
     (⟦aig, ⟨start, inv, h1⟩, projectLeftAssign aig assign⟧ = false)
       →
-    CNF.eval assign ((go aig start h1 (.empty aig)).val.cnf.add (CNF.Clause.empty.add start !inv)) = false := by
+    CNF.eval assign ((go aig start (.of inv) h1 (.empty aig)).val.cnf.add (CNF.Clause.empty.add start !inv)) = false := by
   intro h
-  match heval1:(go aig start h1 (State.empty aig)).val.cnf.eval assign with
+  match heval1 : (go aig start (.of inv) h1 (State.empty aig)).val.cnf.eval assign with
   | true =>
-    have heval2 := (go aig start h1 (.empty aig)).val.cache.inv
-    specialize heval2 assign heval1 start h1 go_marks
-    cases inv <;> simp_all
+    simp
+    intro hassign
+    have heval2 := (go aig start (.of inv) h1 (.empty aig)).val.cache.inv
+    specialize heval2 assign heval1 start inv h1 (BiMark.has_of_le go_marks (by simp))
+    simp [hassign, show ∀ b, true ≤ b ↔ b by decide, h] at heval2
   | false =>
     simp [heval1]
 
@@ -894,7 +1487,7 @@ public theorem toCNF_equisat (entry : Entrypoint Nat) : (toCNF entry).Unsat ↔ 
   simp only [toCNF]
   constructor
   · intro h assign1
-    apply toCNF.go_as_denote
+    apply toCNF.go_as_denote (mark := .of entry.ref.invert)
     specialize h (toCNF.cnfSatAssignment entry.aig assign1)
     rcases entry with ⟨_, ⟨_, _ | _, hgate⟩⟩ <;> simpa [hgate] using h
   · intro h assign
